revm: add test for MUL and DIV

RocqOfRust/revm/revm_interpreter/instructions/simulate/arithmetic.v
@@ -71,6 +71,23 @@ Proof.
   apply Run.Pure.
 Qed.
 
+Definition mul
+    {WIRE : Set} `{Link WIRE}
+    {WIRE_types : InterpreterTypes.Types.t} `{InterpreterTypes.Types.AreLinks WIRE_types}
+    `{!InterpreterTypes.C WIRE_types}
+    (interpreter : Interpreter.t WIRE WIRE_types) :
+    Interpreter.t WIRE WIRE_types :=
+  gas_macro interpreter constants.LOW id (fun interpreter =>
+  popn_top_macro interpreter {| Integer.value := 1 |} id (fun arr top interpreter =>
+    let '{| ArrayPair.x := op1 |} := arr.(array.value) in
+    let op2 := top.(RefStub.projection) interpreter.(Interpreter.stack) in
+    let stack :=
+      top.(RefStub.injection)
+        interpreter.(Interpreter.stack) (Impl_Uint.wrapping_mul op1 op2) in
+    interpreter
+      <| Interpreter.stack := stack |>
+  )).
+
 Lemma mul_eq
     {WIRE H : Set} `{Link WIRE} `{Link H}
     {WIRE_types : InterpreterTypes.Types.t} `{InterpreterTypes.Types.AreLinks WIRE_types}
@@ -90,22 +107,14 @@ Lemma mul_eq
     (
       Output.Success tt,
       [
-        gas_macro interpreter constants.LOW id (fun interpreter =>
-        popn_top_macro interpreter {| Integer.value := 1 |} id (fun arr top interpreter =>
-          let '{| ArrayPair.x := op1 |} := arr.(array.value) in
-          let op2 := top.(RefStub.projection) interpreter.(Interpreter.stack) in
-          let stack :=
-            top.(RefStub.injection)
-              interpreter.(Interpreter.stack) (Impl_Uint.wrapping_mul op1 op2) in
-          interpreter
-            <| Interpreter.stack := stack |>
-        ));
+        mul interpreter;
         _host
       ]%stack
     )
   }}.
 Proof.
   intros.
+  unfold mul.
   gas_macro_eq InterpreterTypesEq.
   popn_top_macro_eq InterpreterTypesEq.
   cbn.
@@ -174,6 +183,27 @@ Proof.
   apply Run.Pure.
 Qed.
 
+Definition div
+    {WIRE : Set} `{Link WIRE}
+    {WIRE_types : InterpreterTypes.Types.t} `{InterpreterTypes.Types.AreLinks WIRE_types}
+    `{!InterpreterTypes.C WIRE_types}
+    (interpreter : Interpreter.t WIRE WIRE_types) :
+    Interpreter.t WIRE WIRE_types :=
+  gas_macro interpreter constants.LOW id (fun interpreter =>
+  popn_top_macro interpreter {| Integer.value := 1 |} id (fun arr top interpreter =>
+    let '{| ArrayPair.x := op1 |} := arr.(array.value) in
+    let op2 := top.(RefStub.projection) interpreter.(Interpreter.stack) in
+    if Impl_Uint.is_zero op2 then
+      interpreter
+    else
+      let stack :=
+        top.(RefStub.injection)
+          interpreter.(Interpreter.stack)
+          (Impl_Uint.wrapping_div op1 op2) in
+      interpreter
+        <| Interpreter.stack := stack |>
+  )).
+
 Lemma div_eq
     {WIRE H : Set} `{Link WIRE} `{Link H}
     {WIRE_types : InterpreterTypes.Types.t} `{InterpreterTypes.Types.AreLinks WIRE_types}
@@ -193,26 +223,14 @@ Lemma div_eq
     (
       Output.Success tt,
       [
-        gas_macro interpreter constants.LOW id (fun interpreter =>
-        popn_top_macro interpreter {| Integer.value := 1 |} id (fun arr top interpreter =>
-          let '{| ArrayPair.x := op1 |} := arr.(array.value) in
-          let op2 := top.(RefStub.projection) interpreter.(Interpreter.stack) in
-          if Impl_Uint.is_zero op2 then
-            interpreter
-          else
-            let stack :=
-              top.(RefStub.injection)
-                interpreter.(Interpreter.stack)
-                (Impl_Uint.wrapping_div op1 op2) in
-            interpreter
-              <| Interpreter.stack := stack |>
-        ));
+        div interpreter;
         _host
       ]%stack
     )
   }}.
 Proof.
   intros.
+  unfold div.
   gas_macro_eq InterpreterTypesEq.
   popn_top_macro_eq InterpreterTypesEq.
   cbn.
